Flypitch.lean
@@ -1,4 +1,5 @@
 import Flypitch.Compat.Core
 import Flypitch.FOL
 import Flypitch.Compactness
+import Flypitch.Completion
 import Flypitch.Examples.Abel
