Flypitch/FOL.lean
@@ -2,3 +2,4 @@ import Flypitch.FOL.Syntax
 import Flypitch.FOL.Formula
 import Flypitch.FOL.Proof
 import Flypitch.FOL.Semantics
+import Flypitch.FOL.Theory
